generic/Zeta.AppSimulate.Helper.fst
@@ -1,0 +1,99 @@
+module Zeta.AppSimulate.Helper
+
+let app_state_feq_implies_equal (#adm:_) (st1 st2: app_state adm)
+  : Lemma (requires (app_state_feq st1 st2))
+          (ensures (st1 == st2))
+  = admit()
+
+let refs_comp (#app:_) (fc: appfn_call app) (k: app_key app.adm)
+  : b:bool { b <==> refs fc k }
+  = admit()
+
+(* for a referenced key, return the parameter position index *)
+let refkey_idx (#app:_) (fc: appfn_call app) (k: app_key app.adm{fc `refs` k})
+  : i:_{let k',v = FStar.Seq.index fc.inp_c i in k' = k}
+  = admit()
+
+let refs_witness (#app:_) (fc: appfn_call app) (k: app_key app.adm)
+ (i: Zeta.SeqAux.seq_index fc.inp_c {k = fst (FStar.Seq.index fc.inp_c i)})
+ = admit()
+
+let input_correct_is_input_consistent (#app:_) (fc: appfn_call app) (st: app_state app.adm)
+  : Lemma (ensures (let rs = fc.inp_c in
+                   input_consistent fc st <==> input_correct st rs))
+  = admit()
+
+let correct_succeeds_if_input_consistent (#app:_) (fc: appfn_call app) (st: app_state app.adm)
+  : Lemma (ensures (succeeds fc st <==> correct fc /\ input_consistent fc st))
+  = admit()
+
+let lemma_post_state (#app:_) (fc: appfn_call app) (st: app_state app.adm {succeeds fc st}) (k: app_key app.adm)
+  : Lemma (ensures (let stpost = apply_trans fc st in
+                    (* fc references k and the value of k in stpost is the written value *)
+                    fc `refs` k /\ write fc k = stpost k
+                      \/
+                    ~ (fc `refs` k) /\ stpost k = st k))
+  = admit()
+
+let prefix_of_valid_valid (#app:_) (fs: seq (appfn_call app) {valid fs}) (i: nat {i <= length fs})
+  : Lemma (ensures (valid (prefix fs i)))
+  = admit()
+
+let lemma_apply_trans (#app:_) (fs: seq (appfn_call app) {length fs > 0 /\ valid fs})
+  : Lemma (ensures (let fs' = hprefix fs in
+                    let fc = telem fs in
+                    post_state fs == apply_trans fc (post_state fs')))
+  = admit()
+
+let lemma_valid_empty (#app:_) (fs: seq (appfn_call app){length fs = 0})
+  : Lemma (ensures (valid fs))
+  = admit()
+
+let lemma_init_value_null (#app:_) (fs: seq (appfn_call app){length fs = 0}) (k: app_key app.adm)
+  : Lemma (ensures (post_state fs k = Null))
+  = admit()
+
+let empty_call_result_valid (#app:_) (rs: seq (appfn_call_res app))
+  : Lemma (ensures (length rs = 0 ==> valid_call_result rs))
+  = admit()
+
+let app_fcs_empty (#app:_) (fcrs: seq (appfn_call_res app))
+  : Lemma (ensures (length fcrs = 0 ==> length (app_fcs fcrs) = 0))
+   = ()
+
+let app_fcs_snoc (#app:_) (fcrs: seq (appfn_call_res app) {length fcrs > 0})
+  : Lemma (ensures (let i = length fcrs - 1 in
+                    let fcrs' = prefix fcrs i in
+                    let fc = to_app_fc fcrs i in
+                    app_fcs fcrs = append1 (app_fcs fcrs') fc))
+  = let i = length fcrs - 1 in
+    let fcrs' = prefix fcrs i in
+    let fcs = app_fcs fcrs in
+    let fcs' = app_fcs fcrs' in
+    let fc = to_app_fc fcrs i in
+    let fcs2 = append1 fcs' fc in
+    let aux (i:_)
+      : Lemma (ensures (index fcs i = index fcs2 i))
+      = ()
+    in
+    FStar.Classical.forall_intro aux;
+    assert(equal fcs fcs2)
+
+let valid_call_result_snoc (#app:_) (fcrs: seq (appfn_call_res app) {length fcrs > 0})
+  : Lemma (requires (let i = length fcrs - 1  in
+                     let fcrs' = prefix fcrs i in
+                     valid_call_result fcrs'))
+          (ensures (let i = length fcrs - 1 in
+                    let fcrs' = prefix fcrs i in
+                    let fcs' = app_fcs fcrs' in
+                    let st' = post_state fcs' in
+                    let fc = to_app_fc fcrs i in
+                    let fcr = index fcrs i in
+                    succeeds fc st' ==>
+                    fcr.res_cr = result fc ==>
+                    valid_call_result fcrs))
+  = admit()
+
+let distinct_keys_comp (#app:_) (sk: FStar.Seq.seq (app_record app))
+  : b:bool {b <==> distinct_keys sk}
+  = admit()
