generic/Zeta.AppSimulate.fst
@@ -1,0 +1,18 @@
+module Zeta.AppSimulate
+
+let prefix_of_distinct_distinct
+  (#adm: app_data_model)
+  (sk: S.seq (app_record adm) {distinct_keys #adm sk})
+  (i: nat { i <= S.length sk }) :
+  Lemma (ensures (let sk' = SA.prefix sk i in
+                  distinct_keys #adm sk'))
+  = admit()
+
+let input_correct (#adm: app_data_model)
+  (st: app_state adm)
+  (inp: S.seq (app_record adm))
+  : Tot (b: bool{b <==>
+                (forall (i: SA.seq_index inp).
+                    let k,v = S.index inp i in
+                    st k = v)})
+  = admit()
