generic/Zeta.Generic.Blum.fst
@@ -1,0 +1,187 @@
+module Zeta.Generic.Blum
+
+let add_il (#vspec #n:_) (ep: epoch) (il: verifiable_log vspec n)
+  : interleaving (ms_hashfn_dom vspec.app) n
+  = admit()
+
+let evict_il (#vspec #n:_) (ep: epoch) (il: verifiable_log vspec n)
+  : interleaving (ms_hashfn_dom vspec.app) n
+  = admit()
+
+let lemma_add_evict_set_identical_glog (#vspec #n:_) (epmax: epoch) (il: verifiable_log vspec n)
+  : Lemma (ensures (aems_equal_upto epmax il <==> G.aems_equal_upto epmax (to_glog il)))
+  = admit()
+
+let add_set_contains_each_add_elem (#vspec #n:_) (il: verifiable_log vspec n) (i: seq_index il{is_blum_add il i})
+  : Lemma (ensures (let be = blum_add_elem il i in
+                    let ep = be.t.e in
+                    add_set ep il `contains` be))
+  = admit()
+
+let some_add_elem_idx
+  (#vspec #n:_)
+  (il: verifiable_log vspec n)
+  (be: ms_hashfn_dom vspec.app {let ep = be.t.e in
+                                add_set ep il `contains` be})
+  : i: seq_index il {is_blum_add il i /\ be = blum_add_elem il i}
+  = admit()
+
+let evict_set_contains_each_evict_elem (#vspec #n:_) (il: verifiable_log vspec n) (i: seq_index il{is_blum_evict il i})
+  : Lemma (ensures (let be = blum_evict_elem il i in
+                    let ep = be.t.e in
+                    evict_set ep il `contains` be))
+  = admit()
+
+let evict_set_is_a_set (#vspec #n:_) (ep: epoch) (il: verifiable_log vspec n)
+  : Lemma (ensures (is_set (evict_set ep il)) )
+  = admit()
+
+let evict_elem_idx
+  (#vspec #n:_)
+  (il: verifiable_log vspec n)
+  (be: ms_hashfn_dom vspec.app {let ep = be.t.e in
+                                evict_set ep il `contains` be})
+  : i: seq_index il {is_blum_evict il i /\ be = blum_evict_elem il i}
+  = admit()
+
+let lemma_evict_before_add (#vspec #n:_) (itsl: its_log vspec n) (i:seq_index itsl{is_blum_add itsl i}):
+  Lemma (ensures (let be = blum_add_elem itsl i in
+                  let ep = be.t.e in
+                  not (evict_set ep itsl `contains` be) \/
+                  evict_elem_idx itsl be < i))
+ = admit()
+
+(* a slightly different version of of the previous lemma - the count of an add element
+ * in the evict set is the same in the prefix as the full sequence *)
+let lemma_evict_before_add2
+  (#vspec #n:_)
+  (ep: epoch)
+  (itsl: its_log vspec n)
+  (i:nat{i <= length itsl})
+  (be: ms_hashfn_dom vspec.app)
+  : Lemma (requires (let itsli = prefix itsl i in
+                     let as = add_set ep itsli in
+                     let es = evict_set ep itsli in
+                     mem be as > mem be es))
+          (ensures (let as = add_set ep itsl in
+                    let es = evict_set ep itsl in
+                    mem be as > mem be es))
+  = admit()
+
+let lemma_evict_before_add3 (#vspec #n:_) (itsl: its_log vspec n) (i: seq_index itsl) (j:seq_index itsl):
+  Lemma (requires (is_blum_add itsl i /\
+                   is_blum_evict itsl j /\
+                   blum_add_elem itsl i = blum_evict_elem itsl j))
+        (ensures (j < i))
+  = admit()
+
+let lemma_add_set_mem (#vspec #n:_) (il: verifiable_log vspec n) (i1 i2: seq_index il)
+  : Lemma (requires (i1 <> i2 /\ is_blum_add il i1 /\ is_blum_add il i2 /\
+                     blum_add_elem il i1 = blum_add_elem il i2))
+          (ensures (let be = blum_add_elem il i1 in
+                    let ep = be.t.e in
+                    mem be (add_set ep il) >= 2))
+  = admit()
+
+(* add elements of a specific key*)
+let k_add_il (#vspec: verifier_spec) (#n:_) (ep: epoch) (gk: key vspec.app) (il: verifiable_log vspec n)
+  : interleaving (ms_hashfn_dom vspec.app) n
+  = admit()
+
+let k_evict_il (#vspec: verifier_spec) (#n:_) (ep: epoch) (gk: key vspec.app) (il: verifiable_log vspec n)
+  : interleaving (ms_hashfn_dom vspec.app) n
+  = admit()
+
+
+let add_set_rel_k_add_set
+  (#vspec: verifier_spec)
+  (#n:_)
+  (ep: epoch)
+  (gk: key vspec.app)
+  (il: verifiable_log vspec n)
+  (be: ms_hashfn_dom vspec.app {let gkc,_ = be.r in gkc = gk})
+  : Lemma (ensures (mem be (k_add_set ep gk il) = mem be (add_set ep il)))
+  = admit()
+
+let evict_set_rel_k_evict_set
+  (#vspec: verifier_spec)
+  (#n:_)
+  (ep: epoch)
+  (gk: key vspec.app)
+  (il: verifiable_log vspec n)
+  (be: ms_hashfn_dom vspec.app{let gkc,_ = be.r in gkc = gk})
+  : Lemma (ensures (mem be (k_evict_set ep gk il) = mem be (evict_set ep il)))
+  = admit()
+
+let k_add_set_correct
+  (#vspec: verifier_spec)
+  (#n:_)
+  (ep: epoch)
+  (gk: key vspec.app)
+  (il: verifiable_log vspec n {length il > 0})
+  (be: ms_hashfn_dom vspec.app)
+  : Lemma (ensures (let gkc,_ = be.r in
+                    k_add_set ep gk il `contains` be ==> gkc = gk /\ be.t.e = ep))
+  = admit()
+
+let k_evict_set_correct
+  (#vspec: verifier_spec)
+  (#n:_)
+  (ep: epoch)
+  (gk: key vspec.app)
+  (il: verifiable_log vspec n {length il > 0})
+  (be: ms_hashfn_dom vspec.app)
+  : Lemma (ensures (let gkc,_ = be.r in
+                    k_evict_set ep gk il `contains` be ==> gkc = gk /\ be.t.e = ep))
+  = admit()
+
+let k_add_set_empty
+  (#vspec: verifier_spec)
+  (#n:_)
+  (ep: epoch)
+  (gk: key vspec.app)
+  (il: verifiable_log vspec n {length il = 0})
+  : Lemma (ensures (k_add_set ep gk il == empty))
+  = admit()
+
+(* if the tail element is a blum add, then the add set is obtained by adding that
+ * blum add to the prefix *)
+let k_add_set_snoc
+  (#vspec: verifier_spec)
+  (#n:_)
+  (ep: epoch)
+  (gk: key vspec.app)
+  (il: verifiable_log vspec n {length il > 0})
+  : Lemma (ensures (let n = length il in
+                    let il' = prefix il (n- 1 ) in
+                    let b = is_blum_add_of_key ep gk il (n - 1) in
+                    let as' = k_add_set ep gk il' in
+                    let as = k_add_set ep gk il in
+                    (b ==> as == add_elem as' (blum_add_elem il (n - 1))) /\
+                    (~b ==> as == as')))
+  = admit()
+
+let k_evict_set_empty
+  (#vspec: verifier_spec)
+  (#n:_)
+  (ep: epoch)
+  (gk: key vspec.app)
+  (il: verifiable_log vspec n {length il = 0})
+  : Lemma (ensures (k_evict_set ep gk il == empty))
+  = admit()
+
+(* analogous theorem for evict sets*)
+let k_evict_set_snoc
+  (#vspec: verifier_spec)
+  (#n:_)
+  (ep: epoch)
+  (gk: key vspec.app)
+  (il: verifiable_log vspec n {length il > 0})
+  : Lemma (ensures (let n = length il in
+                    let il' = prefix il (n- 1 ) in
+                    let b = is_blum_evict_of_key ep gk il (n - 1) in
+                    let as' = k_evict_set ep gk il' in
+                    let as = k_evict_set ep gk il in
+                    (b ==> as == add_elem as' (blum_evict_elem il (n - 1))) /\
+                    (~b ==> as == as')))
+  = admit()
